pulse/lib/core/PulseCore.Atomic.fsti
@@ -308,13 +308,13 @@ val implies_elim (p: slprop) (q: slprop { implies p q })
 : stt_ghost unit emp_inames p (fun _ -> q)
 
 val pers_dup_g (p: slprop)
-  : stt_ghost unit emp_inames (Sep.pers p) (fun _ -> Sep.star (Sep.pers p) (Sep.pers p))
+  : stt_ghost unit emp_inames (pers p) (fun _ -> pers p ** pers p)
 
 val pers_elim_g (p: slprop)
-  : stt_ghost unit emp_inames (Sep.pers p) (fun _ -> p)
+  : stt_ghost unit emp_inames (pers p) (fun _ -> p)
 
 val pers_intro_pure_g (phi: prop)
-  : stt_ghost unit emp_inames (Sep.pure phi) (fun _ -> Sep.pers (Sep.pure phi))
+  : stt_ghost unit emp_inames (pure phi) (fun _ -> pers (pure phi))
 
 val pers_intro_inv_g (i: iref) (p: slprop)
   : stt_ghost unit emp_inames (Sep.inv i p) (fun _ -> Sep.pers (Sep.inv i p))
