pulse/lib/core/PulseCore.InstantiatedSemantics.fsti
@@ -50,6 +50,11 @@ val later_credit_zero () : Lemma (later_credit 0 == emp)
 [@@ erasable]
 val iref : Type0
 val inv (i:iref) (p:slprop) : slprop
+val pers (p: slprop) : slprop
+val pers_dup (p: slprop) : Lemma (implies (pers p) (pers p ** pers p))
+val pers_elim (p: slprop) : Lemma (implies (pers p) p)
+val pers_pure (phi: prop) : Lemma (implies (pure phi) (pers (pure phi)))
+val pers_intro_inv (i: iref) (p: slprop) : Lemma (implies (inv i p) (pers (inv i p)))
 
 val slprop_equiv (p q:slprop) : prop
 
